Functional specification for Model.PNE.decrypt

src/Model.PNE.fsti
@@ -39,9 +39,9 @@ let protected_bits: Type0 = LowParse.BitFields.ubitfield 5 5
 // Note: the sample is PUBLIC so is using QUIC.Spec.lbytes which do not operate over secret integers.
 let sample_length = 16
 let sample = QUIC.Spec.lbytes sample_length
-let pne_plain_length = l:nat {l >= 2 /\ l <= 5}
+let pne_plain_length = l:nat {l >= 1 /\ l <= 4}
 let pne_cipher (l:pne_plain_length) = lbytes l & protected_bits
-let pne_cipherpad = lbytes 5
+let pne_cipherpad = lbytes 5 & protected_bits
 
 /// Restrict a generated cipherpad to the length of the encoded packet number.
 val clip_cipherpad : (cp:pne_cipherpad) -> (l:pne_plain_length) -> pne_cipher l
@@ -49,12 +49,15 @@ val clip_cipherpad : (cp:pne_cipherpad) -> (l:pne_plain_length) -> pne_cipher l
 // We define a separate package type here (different from the one in AEAD). We
 // idealize them separately, and there's a specific part here that's about the
 // protected bits of the header.
+//
+// JP: why is pne_plain_pkg not parameterized over an id type and safe predicate?
 noeq type pne_plain_pkg =
   | PNEPlainPkg:
     pne_plain: (j:id -> l:pne_plain_length -> t:eqtype) ->
     as_bytes: (j:id -> l:pne_plain_length -> pne_plain j l -> GTot (lbytes l & protected_bits)) ->
     repr: (j:unsafe_id -> l:pne_plain_length -> n:pne_plain j l ->
       Tot (b:(lbytes l & protected_bits) {b == as_bytes j l n})) ->
+    mk: (j:unsafe_id -> l:pne_plain_length -> n:lbytes l -> b:protected_bits -> p:pne_plain j l { as_bytes j l p == (n, b) }) ->
     pne_plain_pkg
 
 noeq type info' = {
@@ -104,6 +107,11 @@ val frame_table: #j:safe_id -> #u:info j -> st:pne_state u ->
       r `B.loc_disjoint` (footprint st))
     (ensures table st h1 == table st h0)
 
+// Equality for the pair of (pne, protected_bits) we manipulate in this module.
+let pne_bits_eq #l (x y: pne_cipher l) =
+  fst x `lbytes_eq` fst y && snd x = snd y
+
+// Finding the entry for a given sample.
 let sample_filter (#j:id) (u:info j) (s:sample) (e:entry u) : bool =
   Entry?.s e = s
 
@@ -111,18 +119,18 @@ let entry_for_sample (#j:id) (#u:info j) (s:sample) (st:pne_state u) (h:mem) :
   GTot (option (entry u)) =
   Seq.find_l (sample_filter u s) (table st h)
 
+/// XXX unused
+let contains_sample (#j:id) (#u:info j) (s:sample) (st:pne_state u) (h:mem) :
+  GTot bool =
+  Some? (entry_for_sample s st h)
+
 let fresh_sample (#j:id) (#u:info j) (s:sample) (st:pne_state u) (h:mem) :
   GTot bool =
   None? (entry_for_sample s st h)
 
-let find_sample (#j:id) (#u:info j) (s:sample) (st:pne_state u) (h:mem) :
-  GTot bool =
-  Some? (entry_for_sample s st h)
-
-// Equality for the pair of (pne, protected_bits) we manipulate in this module.
-let pne_bits_eq #l (x y: pne_cipher l) =
-  fst x `lbytes_eq` fst y && snd x = snd y
-
+// Finding the entry for a given cipher. Insofar as I understand, the table
+// keeps a map from plain to cipher (i.e. cipher truncated to the right length,
+// or "clipped"). XXX this seems to be unused.
 let sample_cipher_filter (j:id) (u:info j) (s:sample) (#l:pne_plain_length) (c:pne_cipher l) (e:entry u) : bool =
   Entry?.s e = s && Entry?.l e = l && Entry?.c e `pne_bits_eq` c
 
@@ -130,10 +138,15 @@ let entry_for_sample_cipher (#j:id) (#u:info j) (s:sample) (#l:pne_plain_length)
   GTot (option (entry u)) =
   Seq.find_l (sample_cipher_filter j u s #l c) (table st h)
 
-let find_sample_cipher (#j:id) (#u:info j) (s:sample) (#l:pne_plain_length) (c:pne_cipher l) (st:pne_state u) (h:mem) :
+let contains_sample_cipher (#j:id) (#u:info j) (s:sample) (#l:pne_plain_length) (c:pne_cipher l) (st:pne_state u) (h:mem) :
   GTot bool =
   Some? (entry_for_sample_cipher s #l c st h)
 
+// However, for decryption, we are given a "cipherpad", which should probably be
+// named "padded_cipher". Such a padded cipher may be too long, so what we do
+// instead is define a successful table lookup is a match on i) the protected
+// bits, ii) the sample and iii) the truncation of the cipher. XXX this seems to
+// be unused as well.
 let sample_cipherpad_filter (#j:id) (#u:info j) (s:sample) (cp:pne_cipherpad) (e:entry u) : bool =
   Entry?.s e = s && clip_cipherpad cp (Entry?.l e) `pne_bits_eq` Entry?.c e
 
@@ -141,9 +154,12 @@ let entry_for_sample_cipherpad (#j:id) (#u:info j) (s:sample) (cp:pne_cipherpad)
   GTot (option (entry u)) =
   Seq.find_l (sample_cipherpad_filter s cp) (table st h)
 
-let find_sample_cipherpad (#j:id) (#u:info j) (s:sample) (cp:pne_cipherpad) (st:pne_state u) (h:mem) :
+let contains_sample_cipherpad (#j:id) (#u:info j) (s:sample) (cp:pne_cipherpad) (st:pne_state u) (h:mem) :
   GTot bool =
   Some? (entry_for_sample_cipherpad s cp st h)
+
+/// Stateful API
+/// ------------
 
 val create (j:id) (u:info j) : ST (pne_state u)
   (requires fun _ -> True)
@@ -170,10 +186,10 @@ val encrypt :
     l >= pn_length + 1 /\
     fresh_sample s st h0)
   (ensures fun h0 c h1 ->
-    B.modifies (footprint st) h0 h1 /\
-    (is_safe j ==>
-      table st h1 == Seq.snoc (table st h0) (Entry s #l n c)) /\
-    (~(is_safe j) ==> (
+    B.modifies (footprint st) h0 h1 /\ (
+    if is_safe j then
+      table st h1 == Seq.snoc (table st h0) (Entry s #l n c)
+    else
       let open QUIC.Spec.Lemmas in
       // Our input is: plain packet number, plain bits to be protected
       let pn, bits = PNEPlainPkg?.as_bytes u.plain j l n in
@@ -194,7 +210,6 @@ val encrypt :
       let mask_bits: protected_bits = LowParse.BitFields.get_bitfield (UInt8.v (Seq.index mask 0)) 0 5 in
       let protected_bits = mask_bits `FStar.UInt.logxor` bits in
       return_pn == encrypted_pn /\ return_bits == protected_bits))
-  )
 
 val decrypt :
   (#j:id) ->
@@ -202,14 +217,34 @@ val decrypt :
   (st:pne_state u) ->
   (cp:pne_cipherpad) ->
   (s:sample) ->
-  ST (l:pne_plain_length & pne_plain u l)
+  ST (option(l:pne_plain_length & pne_plain u l))
   (requires fun h0 -> True)
-  (ensures fun h0 (|l, n|) h1 ->
-    modifies_none h0 h1 /\
-    ((is_safe j /\ find_sample s st h0) ==>
-     (match entry_for_sample s st h0 with
-        | Some (Entry _ #l' n' c') ->
-        (l = l' /\ n = n') <==>
-        (l = l' /\ c' `lbytes_eq` clip_cipherpad cp l))
-    )
-  )
+  (ensures fun h0 r h1 ->
+    modifies_none h0 h1 /\ (
+    if is_safe j then
+      match entry_for_sample s st h0 with
+      | None -> None? r
+      | Some (Entry _ #l' n' c') -> Some? r /\ (
+          let Some (| l, n |) = r in
+          (l = l' /\ n = n') <==>
+          (l = l' /\ c' `pne_bits_eq` clip_cipherpad cp l))
+    else
+      let cipher, encrypted_bits = cp in
+      // This mimics the specification of header_decrypt_aux starting after:
+      // let sample = ...
+      let mask = QUIC.Spec.block_of_sample u.calg (key st h0) s in
+      // Decrypting protected bits
+      let mask_bits: protected_bits = LowParse.BitFields.get_bitfield (UInt8.v (Seq.index mask 0)) 0 5 in
+      let bits = mask_bits `FStar.UInt.logxor` encrypted_bits in
+      // Moving on to the pn length which is part of the protected bits
+      let pn_len = LowParse.BitFields.get_bitfield bits 0 2 in
+      assert (0 <= pn_len /\ pn_len <= 3);
+      let pnmask = QUIC.Spec.Lemmas.and_inplace (Seq.slice mask 1 (pn_len + 2)) (QUIC.Spec.pn_sizemask_naive pn_len) 0 in
+      assert (let l = Seq.length pnmask in 1 <= l /\ l <= 4);
+      // Classify, because HACL* specs require secret integers.
+      let pnmask = Seq.init (Seq.length pnmask) (fun i -> Lib.IntTypes.u8 (UInt8.v (Seq.index pnmask i))) in
+      let cipher = Seq.slice cipher 0 (pn_len + 1) in
+      assert (Seq.length cipher == Seq.length pnmask /\ Seq.length cipher == pn_len + 1);
+      let pn = QUIC.Spec.Lemmas.pointwise_op (Lib.IntTypes.(logxor #U8 #SEC)) cipher pnmask 0 in
+      r == Some (| pn_len + 1, PNEPlainPkg?.mk u.plain j (pn_len + 1) pn bits |)
+  ))
